Add eval1

new-semantics/coq/.CoqMakefile.d
@@ -7,9 +7,18 @@ basics/tactics.vos basics/tactics.vok basics/tactics.required_vos: basics/tactic
 theories/Defs.vo theories/Defs.glob theories/Defs.v.beautified theories/Defs.required_vo: theories/Defs.v basics/Basics.vo
 theories/Defs.vio: theories/Defs.v basics/Basics.vio
 theories/Defs.vos theories/Defs.vok theories/Defs.required_vos: theories/Defs.v basics/Basics.vos
+theories/EnvSemantics.vo theories/EnvSemantics.glob theories/EnvSemantics.v.beautified theories/EnvSemantics.required_vo: theories/EnvSemantics.v basics/Basics.vo theories/Defs.vo theories/Syntax.vo theories/SubstFacts.vo
+theories/EnvSemantics.vio: theories/EnvSemantics.v basics/Basics.vio theories/Defs.vio theories/Syntax.vio theories/SubstFacts.vio
+theories/EnvSemantics.vos theories/EnvSemantics.vok theories/EnvSemantics.required_vos: theories/EnvSemantics.v basics/Basics.vos theories/Defs.vos theories/Syntax.vos theories/SubstFacts.vos
 theories/EquivFacts.vo theories/EquivFacts.glob theories/EquivFacts.v.beautified theories/EquivFacts.required_vo: theories/EquivFacts.v basics/Basics.vo theories/Defs.vo theories/SubstFacts.vo
 theories/EquivFacts.vio: theories/EquivFacts.v basics/Basics.vio theories/Defs.vio theories/SubstFacts.vio
 theories/EquivFacts.vos theories/EquivFacts.vok theories/EquivFacts.required_vos: theories/EquivFacts.v basics/Basics.vos theories/Defs.vos theories/SubstFacts.vos
+theories/MemSemantics.vo theories/MemSemantics.glob theories/MemSemantics.v.beautified theories/MemSemantics.required_vo: theories/MemSemantics.v 
+theories/MemSemantics.vio: theories/MemSemantics.v 
+theories/MemSemantics.vos theories/MemSemantics.vok theories/MemSemantics.required_vos: theories/MemSemantics.v 
 theories/SubstFacts.vo theories/SubstFacts.glob theories/SubstFacts.v.beautified theories/SubstFacts.required_vo: theories/SubstFacts.v basics/Basics.vo theories/Defs.vo
 theories/SubstFacts.vio: theories/SubstFacts.v basics/Basics.vio theories/Defs.vio
 theories/SubstFacts.vos theories/SubstFacts.vok theories/SubstFacts.required_vos: theories/SubstFacts.v basics/Basics.vos theories/Defs.vos
+theories/Syntax.vo theories/Syntax.glob theories/Syntax.v.beautified theories/Syntax.required_vo: theories/Syntax.v 
+theories/Syntax.vio: theories/Syntax.v 
+theories/Syntax.vos theories/Syntax.vok theories/Syntax.required_vos: theories/Syntax.v 
