new-semantics/coq/theories/EnvSemantics.v
@@ -1,0 +1,151 @@
+From Basics Require Import Basics.
+From LN Require Import Defs.
+From LN Require Import Syntax.
+From LN Require Import SubstFacts.
+
+Fixpoint read_env {var loc lang} `{Eq var} (σ : nv var loc lang) (x : var) :=
+  match σ with
+  | nv_mt | nv_bloc _ _ _ => None
+  | nv_floc x' _ σ' =>
+    if eqb x x' then None else read_env σ' x
+  | nv_bval x' w σ' =>
+    if eqb x x' then Some w else read_env σ' x
+  end.
+
+Inductive eval1 {var loc} `{Eq var} `{Eq loc} (σ : nv var loc (@val var)): tm -> (vl var loc val) -> Prop :=
+| ev_id x v (READ : read_env σ x = Some (wvl_v v)) : eval1 σ (tm_var x) v
+| ev_rec x v (READ : read_env σ x = Some (wvl_recv v)) : eval1 σ (tm_var x) (open_wvl_vl 0 (wvl_recv v) v)
+| ev_fn x t : eval1 σ (tm_lam x t) (vl_clos (v_fn x t) σ)
+| ev_app t1 t2 x e σ1 v2 v
+  (FN : eval1 σ t1 (vl_clos (v_fn x e) σ1))
+  (ARG : eval1 σ t2 v2)
+  (BODY : eval1 (nv_bval x (wvl_v v2) σ1) e v)
+: eval1 σ (tm_app t1 t2) v
+| ev_link t1 t2 σ1 v
+  (MOD : eval1 σ t1 (vl_exp σ1))
+  (IMP : eval1 σ1 t2 v)
+: eval1 σ (tm_link t1 t2) v
+| ev_mt : eval1 σ tm_mt (vl_exp nv_mt)
+| ev_bind x t1 t2 ℓ v1 σ2
+  (FRESH : ~ In ℓ (floc_nv σ))
+  (BIND : eval1 (nv_floc x ℓ σ) t1 v1)
+  (MOD : eval1 (nv_bval x (wvl_recv (close_vl 0 ℓ v1)) σ) t2 (vl_exp σ2))
+: eval1 σ (tm_bind x t1 t2) (vl_exp (nv_bval x (wvl_recv (close_vl 0 ℓ v1)) σ2))
+.
+
+Lemma read_env_lc {var loc lang} `{Eq var} (σ : nv var loc lang) (Σ : env σ) :
+  forall x w (READ : read_env σ x = Some w), wvalue w.
+Proof.
+  induction σ; ii; ss;
+  des_ifs; eqb2eq var; clarify;
+  inv Σ; eauto.
+Qed.
+
+Lemma eval1_lc {var loc} `{Eq var} `{Name loc} t (σ : nv var loc (@val var)) v (EVAL : eval1 σ t v) :
+  forall (LC : env σ), value v.
+Proof.
+  induction EVAL; ii; ss; eauto.
+  - eapply read_env_lc in READ; eauto. inv READ. auto.
+  - eapply read_env_lc in READ; eauto.
+    inversion READ; clarify.
+    gensym_tac (L ++ floc_vl v) ν.
+    assert (subst_intro_vl _ _ _ v) by eapply subst_intro.
+    rw; eauto.
+    eapply subst_wvl_lc; eauto.
+  - econstructor. auto.
+  - apply IHEVAL3. econstructor.
+    econstructor. apply IHEVAL2. auto.
+    exploit IHEVAL1; eauto. intros LC'.
+    inv LC'. auto.
+  - apply IHEVAL2. exploit IHEVAL1; eauto.
+    intros LC'. inv LC'. auto.
+  - repeat constructor.
+  - assert (wvalue (wvl_recv (close_vl 0 ℓ v1))).
+    econstructor. instantiate (1 := []). ii.
+    assert (close_open_loc_eq_vl _ _ _ v1) by eapply close_open_loc_eq; rw.
+    exploit IHEVAL1; eauto. constructor; auto. intros VAL1.
+    assert (open_loc_lc_vl _ _ _ v1 VAL1) by (eapply open_loc_lc; auto).
+    rw.
+    eapply subst_loc_lc. auto.
+    repeat constructor; eauto.
+    exploit IHEVAL2.
+    constructor; auto.
+    intros VAL. inv VAL. auto.
+Qed.
+
+Lemma read_env_map {var loc lang} `{Eq var} `{Eq loc} (σ : nv var loc lang) :
+  forall φ w x (READ : read_env σ x = Some w),
+    read_env (map_nv φ σ) x = Some (map_wvl φ w).
+Proof.
+  induction σ; ii; ss;
+  des_ifs; ss;
+  des_ifs; eqb2eq var; clarify;
+  try eqb2eq loc; clarify; eauto.
+Qed.
+
+Lemma read_env_floc {var loc lang} `{Eq var} `{Eq loc} (σ : nv var loc lang) :
+  forall w ℓ x (READ : read_env σ x = Some w) (IN : In ℓ (floc_wvl w)),
+    In ℓ (floc_nv σ).
+Proof.
+  induction σ; ii; ss;
+  des_ifs; ss;
+  eqb2eq var; clarify; eauto;
+  rewrite in_app_iff; eauto.
+Qed.
+
+Lemma eval1_floc_dec {var loc} `{Eq var} `{Name loc} t (σ : nv var loc (@val var)) v (EVAL : eval1 σ t v) :
+  forall ℓ (IN : In ℓ (floc_vl v)), In ℓ (floc_nv σ).
+Proof.
+  induction EVAL; ii; ss; eauto.
+  - eapply read_env_floc; eauto.
+  - gensym_tac (floc_vl v) ν.
+    assert (subst_intro_vl _ _ _ v) as RR by eapply subst_intro.
+    rewrite RR in IN; eauto.
+    assert (floc_subst_wvl_vl _ _ _ (open_loc_vl 0 ν v)) as HINT by eapply floc_subst_wvl.
+    apply HINT in IN.
+    des; ss.
+    apply open_floc in IN0. des; clarify.
+    eapply read_env_floc; eauto.
+    eapply read_env_floc; eauto.
+  - apply IHEVAL3 in IN.
+    rewrite in_app_iff in IN; des; eauto.
+  - rewrite in_app_iff in *.
+    des; eauto.
+    eapply close_floc in IN. des.
+    exploit IHEVAL1; eauto. ii; des; clarify.
+    exploit IHEVAL2; eauto. intros IN'.
+    rewrite in_app_iff in *.
+    des; eauto.
+    eapply close_floc in IN'. des.
+    exploit IHEVAL1; eauto. ii; des; clarify.
+Qed.
+
+Lemma eval1_map {var loc} `{Eq var} `{Name loc} t (σ : nv var loc (@val var)) v (EVAL : eval1 σ t v) :
+  forall φ (INJ : forall ℓ ν (fEQ : φ ℓ = φ ν), ℓ = ν),
+    eval1 (map_nv φ σ) t (map_vl φ v).
+Proof.
+  induction EVAL; ii; ss; try solve [econstructor; eauto].
+  - econstructor. exploit (read_env_map σ); eauto.
+  - assert (map_open_wvl_vl _ _ _ v) by (eapply map_open_wvl).
+    rw. eapply ev_rec.
+    exploit (read_env_map σ); eauto.
+  - assert (map_close_vl _ _ _ v1) by (eapply map_close).
+    rw; eauto.
+    econstructor; eauto.
+    red. intros IN. eapply map_floc in IN; eauto.
+    rrw; eauto.
+Qed.
+
+Lemma eval1_subst {var loc} `{Eq var} `{Name loc} t (σ : nv var loc (@val var)) v (EVAL : eval1 σ t v) :
+  forall ℓ' ν (FRESH : ~ In ν (floc_nv σ)),
+    eval1 (subst_loc_nv ν ℓ' σ) t (subst_loc_vl ν ℓ' v).
+Proof.
+  ii. pose proof (eval1_map t σ v EVAL (swap id ν ℓ')) as HINT.
+  assert (swap_is_subst_nv _ _ _ σ) as RR by eapply swap_is_subst.
+  assert (swap_is_subst_vl _ _ _ v) as RR' by eapply swap_is_subst.
+  rewrite <- RR. rewrite <- RR'.
+  apply HINT.
+  ii; unfold swap, id in fEQ; des_ifs; repeat eqb2eq loc; clarify.
+  red. intros IN. eapply eval1_floc_dec in EVAL; eauto.
+  eauto.
+Qed.
